\documentclass[12pt]{article}
\usepackage{amsmath, amssymb}

\title{CS 588: Homework 3}
\author{David Deng}

\begin{document}
\maketitle

\section*{Exercise 9.3}

Let $u$, $v$ be unit vectors such that $au = x$ and $bv = y$ for some $a,b \in \mathbb{R}^+$.
To show 
$$\vert\langle f(x), f(y) \rangle - \langle x,y\rangle \vert \leq \epsilon \|x\|\|y\|$$
it suffices to show
$$\vert\langle f(au), f(bv) \rangle - \langle au,bv\rangle \vert \leq \epsilon ab\|u\|\|v\|$$
Since $f$ is linear, $f(au) = af(u)$ and $f(av) = af(v)$. By property of dot product, we also have $\langle ax, by\rangle = ab\langle x, y\rangle$.
Thus, the above is also equivalent to
$$\vert ab \langle f(u), f(v) \rangle - ab \langle u,v\rangle \vert \leq \epsilon ab\|u\|\|v\|$$
Since $a,b > 0$, and unit vector $\|u\| = \|v\| = 1$, we have
$$ab \vert \langle f(u), f(v) \rangle - \langle u,v\rangle \vert \leq \epsilon ab\|u\|\|v\| = \epsilon$$
and thus showing
$$\vert \langle f(u), f(v) \rangle - \langle u,v\rangle \vert \leq \epsilon$$
is enough to solve this question.

Recall for any vector $x$ and $y$, we have 
$$\|x + y \|^2 = \sum_{i=1}^d (x_i + y_i)^2 = \sum_{i=1}^d x_i^2 + y_i^2 + 2x_iy_i = \|x\|^2 + \|y\|^2 + 2\langle x,y\rangle$$
Similarly,
$$\|x - y \|^2 = \sum_{i=1}^d (x_i - y_i)^2 = \sum_{i=1}^d x_i^2 + y_i^2 - 2x_iy_i = \|x\|^2 + \|y\|^2 - 2\langle x,y\rangle$$
Subtracting the two equations, we have
$$\|x + y \|^2 - \|x - y \|^2 = 4\langle x,y\rangle$$
and thus
$$\langle x,y\rangle = \frac{\|x + y \|^2 - \|x - y \|^2}{4}$$
Using this property, we can simplify the LHS of the equation further:
Let $U = \|f(u)+f(v)\|^2-\|f(u)-f(v)\|^2$, and $V = \|u+v\|^2 - \|u-v\|^2$, 
and let $U' = \|f(u)+f(v)\|^2-\|u+v\|^2$, and $V' = \|f(u)-f(v)\|^2- \|u-v\|^2$, 

We have $U-V = U'-V'$.
\begin{align*}
\vert \langle f(u), f(v) \rangle - \langle u,v\rangle \vert = & \vert\frac{U-V}{4}\vert\\
=& \vert\frac{U'-V'}{4}\vert \\
\leq & \frac{\vert U'\vert + \vert V'\vert}{4} \\
\overset{(a)}{\leq}& \frac{\epsilon (\|u+v\|)^2 + \epsilon (\|u-v\|)^2}{4} \\
=& \frac{2\epsilon (\|u\|^2 + \|v\|^2)}{4} \\
=& \epsilon
\end{align*}
where (a) is by JL, where $\vert U' \vert= \vert \|f(u)+f(v)\|^2-\|u+v\|^2 \vert \leq \epsilon (\|u+v\|)^2$, and $\vert V' \vert= \vert \|f(u)-f(v)\|^2-\|u-v\|^2 \vert \leq \epsilon (\|u-v\|)^2$.

\section*{Exercise 9.4}



\end{document}